wasm: Prove termination of evaluate_wasm

compiler/backend/semantics/wasmSemScript.sml
@@ -36,301 +36,363 @@ val _ = Datatype `
      ; clock: num
      |>`
 
-(* Same as above, but decrements clock. *)
+(* TODO: There are multiple ad-hoc definitions of orderings floating around this file... *)
+
+val code_order = Define `code_order = inv_image ($<) (\c. ainstr2_size (SND c))`
+
 val expand_def = Define `
-expand s vs es =
-      let (vs', es') = s.code in
-          if LENGTH vs < LENGTH vs' \/ LENGTH es > 1 then (* No. instructions does not change, no. results increases. *)
-              if s.clock = 0n then (SOME Timeout, s)
-              else (NONE, s with <| clock := (s.clock - 1n); code := (vs, es ++ (TL es')) |>)
-          else (NONE, s with code := (vs, es ++ (TL es')))`
+  expand s vs es =
+    let c = (vs, es ++ (TL (SND s.code))) in
+      if (ainstr2_size (SND c)) < (ainstr2_size (SND s.code))
+      then (NONE, s with code := c)
+      else
+        if s.clock = 0
+        then (SOME Timeout, s)
+        else (NONE, s with <| code := c; clock := s.clock - 1 |>)`
 
-(* Same as above, but for a singleton instruction (this is more common). *)
+(* Showing that expand ensures some lexicographic order helps for
+ * termination proof of wasm_evaluate below. *)
+val expand_dec = Q.store_thm("expand_dec[simp]",
+  `expand s vs es = (NONE, s') ==> (($< LEX $<) (s'.clock, ainstr2_size (SND s'.code)) (s.clock, ainstr2_size (SND s.code)))`,
+  rw[expand_def] >> simp [expand_def,LEX_DEF] >> rw [expand_def] >> simp [expand_def,LEX_DEF]
+)
+
 val effect_def = Define `effect s vs e = expand s vs [e]`
-
-(* Helper function for executing instructions that only alter the result. *)
 val resulting_def = Define `resulting s vs' = expand s vs' []`
 
-val typ_assert = Define `
+val typ_assert_def = Define `
   typ_assert msg cond (r, s) = ((if cond then r else SOME (TypeError msg)), s)`
 
-val evaluate_nomatch = Define `evaluate_nomatch s = (SOME (TypeError "No reduction rule applicable. Stack does not match."), s)`
+val typ_assert_eq_none = Q.store_thm("typ_assert_eq_none[simp]",
+  `typ_assert msg c p = (NONE, s') <=> c /\ p = (NONE, s')`,
+  Cases_on `p` >> simp [AllCaseEqs (), typ_assert_def] >> metis_tac []
+)
 
-(* NOTE: Traps are not bubbled up through reductions but returned directly! *)
-val evaluate_small_def = Define `
-  evaluate_small s = let (vs, es) = s.code in (case (vs, (HD es)) of
-    | vs, Plain pe => (case (vs, pe) of
+val evaluate_nomatch_def = Define `
+  evaluate_nomatch s = (SOME (TypeError "No reduction rule applicable. Stack does not match."), s)`
 
-      (* 4.4.1  Numeric Instructions *)
-
-      (* 4.4.1.1 *)
-      (* This rule is not in the spec since values are represented by constants there. *)
-      | vs, Const v =>
-        resulting s (v :: vs)
-
-      (* 4.4.1.2 *)
-      | V_i32 c :: vs', Unop_i W32 op =>
-        resulting s ((V_i32 (app_unop_i op c)) :: vs')
-      | V_i64 c :: vs', Unop_i W64 op =>
-        resulting s ((V_i64 (app_unop_i op c)) :: vs')
-      | V_f32 c :: vs', Unop_f W32 op =>
-        resulting s ((V_f32 (app_unop_f op c)) :: vs')
-      | V_f64 c :: vs', Unop_f W64 op =>
-        resulting s ((V_f64 (app_unop_f op c)) :: vs')
-
-      (* 4.4.1.3 *)
-      | V_i32 c1 :: V_i32 c2 :: vs', Binop_i W32 op =>
-        let vop = app_binop_i op c1 c2 in (case vop of
-          | SOME c3 => resulting s (V_i32 c3 :: vs')
-          | NONE    => (SOME (Trap "Undefined result for binary operation on i32"), s)
-        )
-      | V_i64 c1 :: V_i64 c2 :: vs', Binop_i W64 op =>
-        let vop = app_binop_i op c1 c2 in (case vop of
-          | SOME c3 => resulting s (V_i64 c3 :: vs')
-          | NONE    => (SOME (Trap "Undefined result for binary operation on i64"), s)
-        )
-      | V_f32 c1 :: V_f32 c2 :: vs', Binop_f W32 op =>
-        let vop = app_binop_f op c1 c2 in (case vop of
-          | SOME c3 => resulting s (V_f32 c3 :: vs')
-          | NONE    => (SOME (Trap "Undefined result for binary operation on f32"), s)
-        )
-      | V_f64 c1 :: V_f64 c2 :: vs', Binop_f W64 op =>
-        let vop = app_binop_f op c1 c2 in (case vop of
-          | SOME c3 => resulting s (V_f64 c3 :: vs')
-          | NONE    => (SOME (Trap "Undefined result for binary operation on f64"), s)
-        )
-
-      (* 4.4.1.4 *)
-      | V_i32 c :: vs', Testop_i W32 op =>
-        resulting s ((wrap_bool (app_testop_i op c)) :: vs')
-      | V_i64 c :: vs', Testop_i W64 op =>
-        resulting s ((wrap_bool (app_testop_i op c)) :: vs')
-
-      (* 4.4.1.5 *)
-      | V_i32 c1 :: V_i32 c2 :: vs', Relop_i W32 op =>
-        resulting s ((wrap_bool (app_relop_i op c1 c2)) :: vs')
-      | V_i64 c1 :: V_i64 c2 :: vs', Relop_i W64 op =>
-        resulting s ((wrap_bool (app_relop_i op c1 c2)) :: vs')
-      | V_f32 c1 :: V_f32 c2 :: vs', Relop_f W32 op =>
-        resulting s ((wrap_bool (app_relop_f op c1 c2)) :: vs')
-      | V_f64 c1 :: V_f64 c2 :: vs', Relop_f W64 op =>
-        resulting s ((wrap_bool (app_relop_f op c1 c2)) :: vs')
-
-      (* 4.4.1.6 *)
-      | v :: vs', Conversion c =>
-        let vo = cvt c v in (case vo of
-          | SOME v' => resulting s (v' :: vs')
-          | NONE    => (SOME (Trap "Conversion error"), s)
-        )
-
-      (* 4.4.2  Parametric Instructions *)
-
-      (* 4.4.2.1 *)
-      | v :: vs', Drop =>
-        resulting s vs'
-
-      (* 4.4.2.2 *)
-      | V_i32 0w :: v2 :: v1 :: vs', Select =>
-        resulting s (v2 :: vs')
-      | V_i32 i :: v2 :: v1 :: vs', Select =>
-        resulting s (v1 :: vs')
-
-      (* 4.4.3  Variable Instructions *)
-
-      (* 4.4.3.1 *)
-      | vs, Get_local x =>
-        typ_assert "4.4.3.1.2" ((w2n x) < LENGTH s.frame.locals)
-          (resulting s ((EL (w2n x) s.frame.locals) :: vs))
-
-      (* 4.4.3.2 *)
-      | v :: vs', Set_local x =>
-        typ_assert "4.4.3.2.2" ((w2n x) < LENGTH s.frame.locals)
-          (resulting (s with frame := (s.frame with locals := (LUPDATE v (w2n x) s.frame.locals))) vs')
-
-      (* 4.4.3.3 *)
-      | c :: vs', Tee_local x =>
-        (* Stack length remains unchanged, result length increases. *)
-        effect s (c :: c :: vs') (Plain (Set_local x))
-
-      (* 4.4.3.4 *)
-      | vs, Get_global x =>
-        typ_assert "4.4.3.4.2" ((w2n x) < LENGTH s.frame.module.globaladdrs)
-          (let a = EL (w2n x) s.frame.module.globaladdrs in
-             typ_assert "4.4.3.4.4" (a < LENGTH s.store.globals)
-               (resulting s ((EL a s.store.globals).value :: vs))
-          )
-
-      (* 4.4.3.5 *)
-      | v :: vs', Set_global x =>
-        typ_assert "4.4.3.5.2" ((w2n x) < LENGTH s.frame.module.globaladdrs)
-          (let a = EL (w2n x) s.frame.module.globaladdrs in
-            typ_assert "4.4.3.5.4" (a < LENGTH s.store.globals)
-              (let glob = EL a s.store.globals in
-                typ_assert "Cannot set immutable global" (glob.mut = T_var)
-                  (resulting (s with store := (s.store with globals := LUPDATE (glob with value := v) a s.store.globals)) vs')
-              )
-          )
-
-      (* 4.4.4  Memory Instructions *)
-
-      (* 4.4.4.1 *)
-      | i :: vs', Load t ma =>
-        (case mem_load_t s.store s.frame t ma i of
-           | SOME v => resulting s (v :: vs')
-           | NONE   => (SOME (Trap "Bad load instruction"), s)
-        )
-      | i :: vs', Loadi w tp sx ma =>
-        (case mem_load_w_sx s.store s.frame w tp sx ma i of
-           | SOME v => resulting s (v :: vs')
-           | NONE   => (SOME (Trap "Bad load instruction"), s)
-        )
-
-      (* 4.4.4.2 *)
-      (* TODO: Write a store function that avoids unbounded 'a word. *)
-      (* | i :: v :: vs', Store t ma => *)
-      (*   (case mem_store s.store s.frame (bit_width (typeof v)) ma i (val2w v) of *)
-      (*      | SOME s' => resulting (s with store := s') vs' *)
-      (*      | NONE => (SOME (Trap "Bad store instruction"), s)) *)
-
-      (* | i :: v :: vs', Storei w tp ma => *)
-      (*   (case mem_store s.store s.frame (bit_width_p tp) ma i (val2w v) of *)
-      (*      | SOME s' => resulting (s with store := s') vs' *)
-      (*      | NONE => (SOME (Trap "Bad store instruction"), s)) *)
-
-      (* 4.4.4.3 *)
-      | vs, Current_memory =>
-        resulting s ((V_i32 (n2w (bytes_to_pages (LENGTH (get_mem s.store s.frame))))) :: vs)
-
-      (* 4.4.4.4 *)
-      (* NOTE: Growing memory always fails. That matches CakeML and makes it deterministic! *)
-      | n :: vs', Grow_memory =>
-        resulting s ((V_i32 (i2w ~1)) :: vs')
-
-      (* 4.4.5  Control Instructions *)
-
-      (* 4.4.5.1 *)
-      | vs, Nop =>
-        resulting s vs
-
-      (* 4.4.5.2 *)
-      | vs, Unreachable =>
-        (SOME (Trap "Unreachable"), s)
-
-      (* 4.4.5.3 *)
-      | vs, Block ts es' =>
-        (* Same stack and result length, block is swapped for label. *)
-        effect s vs (Label (LENGTH ts) [] ([], (MAP Plain es')))
-
-      (* 4.4.5.4 *)
-      | vs, Loop ts es' =>
-        (* Same stack and result length, loop is swapped for label. *)
-        effect s vs (Label 0 [pe] ([], (MAP Plain es')))
-
-      (* 4.4.5.5 *)
-      | V_i32 0w :: vs', If t i1s i2s =>
-        effect s vs' (Plain (Block t i2s))
-      | V_i32 i :: vs', If t i1s i2s =>
-        effect s vs' (Plain (Block t i1s))
-
-      (* 4.4.5.6 [moved-down] *)
-
-      (* 4.4.5.7 *)
-      | V_i32 0w :: vs', Br_if l =>
-        resulting s vs'
-      | V_i32 i :: vs', Br_if l =>
-        effect s vs' (Plain (Br l))
-
-      (* 4.4.5.8 *)
-      | V_i32 i :: vs', Br_table ls ln =>
-        let nls = to_list ls in
-         effect s vs' (Plain (Br (if w2n i < LENGTH nls then EL (w2n i) nls else ln)))
-
-      (* 4.4.5.9 [moved-down] *)
-
-      (* 4.4.5.10 *)
-      | vs, Call x =>
-        typ_assert "4.4.5.10.2" ((w2n x) < LENGTH s.frame.module.funcaddrs)
-          (effect s vs (Invoke (EL (w2n x) s.frame.module.funcaddrs)))
-
-      (* 4.4.5.11 *)
-      | V_i32 i :: vs', Call_indirect x =>
-        let tab = get_table s.store s.frame in
-          typ_assert "4.4.4.5.11.10" ((w2n x) < LENGTH tab)
-            (case EL (w2n i) tab of
-               | NONE => (SOME (TypeError "4.4.5.11.11"), s)
-               | SOME a =>
-                 typ_assert "4.4.5.11.13" (a < LENGTH s.store.funcs)
-                   if funcinst_type (EL a s.store.funcs) <> (EL (w2n x) s.frame.module.types)
-                   then (SOME (Trap "4.4.5.11.16"), s)
-                   else effect s vs' (Invoke a)
-            )
-
-      | vs, pe =>
-        evaluate_nomatch s
-    )
-
-    (* 4.4.5.6 *)
-    (* TODO: Get rid of fill_b. *)
-    (* | vs, Label (LENGTH vs') is (fill_b l holed (vs', [Plain (Br (n2w l))])) => *)
-    (*   expand s (vs' ++ vs) (MAP Plain is) *)
-
-    (* 4.4.5.9 *)
-    (* TODO: Get rid of fill_b. *)
-    (* | vs, Frame (LENGTH vs') s.frame (fill_b b k (vs', [Plain Return])) => *)
-    (*   resulting s (vs' ++ vs) *)
-
-    (* 4.4.6.2 *)
-    | vs, Label n is (vs', []) =>
-      resulting s (vs' ++ vs)
-
-    (* 4.4.7.{1,3} *)
-    | vs, Invoke a =>
-      typ_assert "4.4.7.1.2" (a <= LENGTH s.store.funcs)
-        (case (EL a s.store.funcs) of
-           (* 4.4.7.1 *)
-           | Native (Tf t1 t2) mi f => (
-             let (n, m) = (LENGTH t1, LENGTH t2) in
-             typ_assert "4.4.7.1.{4,7} (at least one of the two)" (m <= 1 /\ n <= LENGTH vs)
-               (effect s (DROP n vs) (Frame
-                 m
-                 <| module := mi; locals := (TAKE n vs) ++ (MAP zero f.locals) |>
-                 ([], [Plain (Block t2 (expr_to_instrs f.body))])
-               ))
-           )
-
-           (* 4.4.7.3 *)
-           (* NOTE: We assume that any host function is of type [i32] ^ 4 -> []. *)
-           (* TODO: This case explodes. Assert i32^4 separately. *)
-           (* | Host (ForeignFunction name) => (case vs of *)
-           (*   | V_i32 (n2w len2) :: V_i32 (n2w ptr2) :: V_i32 (n2w len1) :: V_i32 (n2w ptr1) :: vs' => *)
-           (*     let rbs = read_mem s.store s.frame in *)
-           (*    case (rbs ptr1 len1, rbs ptr2 len2) of *)
-           (*       | SOME b1s, SOME b2s => (case call_FFI s.ffi name b1s b2s of *)
-           (*         | FFI_final outcome => (SOME (FinalFFI outcome), s) *)
-           (*         | FFI_return new_ffi new_bytes => (case write_mem s.store s.frame ptr1 new_bytes of *)
-           (*           | SOME s' => resulting (s with <| ffi := new_ffi; store := s' |>) vs' *)
-           (*           | NONE    => (SOME (Trap "Host function wants to write out of bounds"), s) *)
-           (*         ) *)
-           (*       ) *)
-           (*       | _ => (SOME (Trap "Host function arguments out of bounds"), s) *)
-           (*   | _ => (SOME (TypeError "Host function expects four i32 arguments"), s) *)
-           (* ) *)
-        )
-
-    (* 4.4.7.2 *)
-    | vs, Frame n f (vs', []) =>
-      resulting s (vs' ++ vs)
-
-    | vs, es =>
-      evaluate_nomatch s
-  )
-`
+val evaluate_nomatch_eq_none = Q.store_thm("evaluate_nomatch_eq_none[simp]",
+  `evaluate_nomatch s <> (NONE, s')`,
+  simp[evaluate_nomatch_def]
+)
 
 val wrap_result = Define `
-  wrap_result l = case LENGTH l of
-    | 0 => Result NONE
-    | 1 => Result (SOME (HD l))
-    | _ => TypeError "Expected result of at most one value"`
+wrap_result l = case LENGTH l of
+                  | 0 => Result NONE
+                  | 1 => Result (SOME (HD l))
+                  | _ => TypeError "Expected result of at most one value"`
+
+(* NOTE: Traps are not bubbled up through reductions but returned directly! *)
+val evaluate_small_def = tDefine "evaluate_small" `
+  evaluate_small s = case s.code of
+    | vs, NIL => (SOME (wrap_result vs), s)
+    | vs, (e::es) => case (vs, e) of
+      | vs, Plain pe => (case (vs, pe) of
+
+        (* 4.4.1  Numeric Instructions *)
+
+        (* 4.4.1.1 *)
+        (* This rule is not in the spec since values are represented by constants there. *)
+        | vs, Const v =>
+          resulting s (v :: vs)
+
+        (* 4.4.1.2 *)
+        | V_i32 c :: vs', Unop_i W32 op =>
+          resulting s ((V_i32 (app_unop_i op c)) :: vs')
+        | V_i64 c :: vs', Unop_i W64 op =>
+          resulting s ((V_i64 (app_unop_i op c)) :: vs')
+        | V_f32 c :: vs', Unop_f W32 op =>
+          resulting s ((V_f32 (app_unop_f op c)) :: vs')
+        | V_f64 c :: vs', Unop_f W64 op =>
+          resulting s ((V_f64 (app_unop_f op c)) :: vs')
+
+        (* 4.4.1.3 *)
+        | V_i32 c1 :: V_i32 c2 :: vs', Binop_i W32 op =>
+          let vop = app_binop_i op c1 c2 in (case vop of
+            | SOME c3 => resulting s (V_i32 c3 :: vs')
+            | NONE    => (SOME (Trap "Undefined result for binary operation on i32"), s)
+          )
+        | V_i64 c1 :: V_i64 c2 :: vs', Binop_i W64 op =>
+          let vop = app_binop_i op c1 c2 in (case vop of
+            | SOME c3 => resulting s (V_i64 c3 :: vs')
+            | NONE    => (SOME (Trap "Undefined result for binary operation on i64"), s)
+          )
+        | V_f32 c1 :: V_f32 c2 :: vs', Binop_f W32 op =>
+          let vop = app_binop_f op c1 c2 in (case vop of
+            | SOME c3 => resulting s (V_f32 c3 :: vs')
+            | NONE    => (SOME (Trap "Undefined result for binary operation on f32"), s)
+          )
+        | V_f64 c1 :: V_f64 c2 :: vs', Binop_f W64 op =>
+          let vop = app_binop_f op c1 c2 in (case vop of
+            | SOME c3 => resulting s (V_f64 c3 :: vs')
+            | NONE    => (SOME (Trap "Undefined result for binary operation on f64"), s)
+          )
+
+        (* 4.4.1.4 *)
+        | V_i32 c :: vs', Testop_i W32 op =>
+          resulting s ((wrap_bool (app_testop_i op c)) :: vs')
+        | V_i64 c :: vs', Testop_i W64 op =>
+          resulting s ((wrap_bool (app_testop_i op c)) :: vs')
+
+        (* 4.4.1.5 *)
+        | V_i32 c1 :: V_i32 c2 :: vs', Relop_i W32 op =>
+          resulting s ((wrap_bool (app_relop_i op c1 c2)) :: vs')
+        | V_i64 c1 :: V_i64 c2 :: vs', Relop_i W64 op =>
+          resulting s ((wrap_bool (app_relop_i op c1 c2)) :: vs')
+        | V_f32 c1 :: V_f32 c2 :: vs', Relop_f W32 op =>
+          resulting s ((wrap_bool (app_relop_f op c1 c2)) :: vs')
+        | V_f64 c1 :: V_f64 c2 :: vs', Relop_f W64 op =>
+          resulting s ((wrap_bool (app_relop_f op c1 c2)) :: vs')
+
+        (* 4.4.1.6 *)
+        | v :: vs', Conversion c =>
+          let vo = cvt c v in (case vo of
+            | SOME v' => resulting s (v' :: vs')
+            | NONE    => (SOME (Trap "Conversion error"), s)
+          )
+
+        (* 4.4.2  Parametric Instructions *)
+
+        (* 4.4.2.1 *)
+        | v :: vs', Drop =>
+          resulting s vs'
+
+        (* 4.4.2.2 *)
+        | V_i32 0w :: v2 :: v1 :: vs', Select =>
+          resulting s (v2 :: vs')
+        | V_i32 i :: v2 :: v1 :: vs', Select =>
+          resulting s (v1 :: vs')
+
+        (* 4.4.3  Variable Instructions *)
+
+        (* 4.4.3.1 *)
+        | vs, Get_local x =>
+          typ_assert "4.4.3.1.2" ((w2n x) < LENGTH s.frame.locals)
+            (resulting s ((EL (w2n x) s.frame.locals) :: vs))
+
+        (* 4.4.3.2 *)
+        | v :: vs', Set_local x =>
+          typ_assert "4.4.3.2.2" ((w2n x) < LENGTH s.frame.locals)
+            (resulting (s with frame := (s.frame with locals := (LUPDATE v (w2n x) s.frame.locals))) vs')
+
+        (* 4.4.3.3 *)
+        | c :: vs', Tee_local x =>
+          (* Stack length remains unchanged, result length increases. *)
+          effect s (c :: c :: vs') (Plain (Set_local x))
+
+        (* 4.4.3.4 *)
+        | vs, Get_global x =>
+          typ_assert "4.4.3.4.2" ((w2n x) < LENGTH s.frame.module.globaladdrs)
+            (let a = EL (w2n x) s.frame.module.globaladdrs in
+              typ_assert "4.4.3.4.4" (a < LENGTH s.store.globals)
+                (resulting s ((EL a s.store.globals).value :: vs))
+            )
+
+        (* 4.4.3.5 *)
+        | v :: vs', Set_global x =>
+          typ_assert "4.4.3.5.2" ((w2n x) < LENGTH s.frame.module.globaladdrs)
+            (let a = EL (w2n x) s.frame.module.globaladdrs in
+              typ_assert "4.4.3.5.4" (a < LENGTH s.store.globals)
+                (let glob = EL a s.store.globals in
+                  typ_assert "Cannot set immutable global" (glob.mut = T_var)
+                    (resulting (s with store := (s.store with globals := LUPDATE (glob with value := v) a s.store.globals)) vs')
+                )
+            )
+
+        (* 4.4.4  Memory Instructions *)
+
+        (* 4.4.4.1 *)
+        | i :: vs', Load t ma =>
+          (case mem_load_t s.store s.frame t ma i of
+            | SOME v => resulting s (v :: vs')
+            | NONE   => (SOME (Trap "Bad load instruction"), s)
+          )
+        | i :: vs', Loadi w tp sx ma =>
+          (case mem_load_w_sx s.store s.frame w tp sx ma i of
+            | SOME v => resulting s (v :: vs')
+            | NONE   => (SOME (Trap "Bad load instruction"), s)
+          )
+
+        (* 4.4.4.2 *)
+        (* TODO: Write a store function that avoids unbounded 'a word. *)
+        (* | i :: v :: vs', Store t ma => *)
+        (*   (case mem_store s.store s.frame (bit_width (typeof v)) ma i (val2w v) of *)
+        (*      | SOME s' => resulting (s with store := s') vs' *)
+        (*      | NONE => (SOME (Trap "Bad store instruction"), s)) *)
+
+        (* | i :: v :: vs', Storei w tp ma => *)
+        (*   (case mem_store s.store s.frame (bit_width_p tp) ma i (val2w v) of *)
+        (*      | SOME s' => resulting (s with store := s') vs' *)
+        (*      | NONE => (SOME (Trap "Bad store instruction"), s)) *)
+
+        (* 4.4.4.3 *)
+        | vs, Current_memory =>
+          resulting s ((V_i32 (n2w (bytes_to_pages (LENGTH (get_mem s.store s.frame))))) :: vs)
+
+        (* 4.4.4.4 *)
+        (* NOTE: Growing memory always fails. That matches CakeML and makes it deterministic! *)
+        | n :: vs', Grow_memory =>
+          resulting s ((V_i32 (i2w ~1)) :: vs')
+
+        (* 4.4.5  Control Instructions *)
+
+        (* 4.4.5.1 *)
+        | vs, Nop =>
+          resulting s vs
+
+        (* 4.4.5.2 *)
+        | vs, Unreachable =>
+          (SOME (Trap "Unreachable"), s)
+
+        (* 4.4.5.3 *)
+        | vs, Block ts es' =>
+          (* Same stack and result length, block is swapped for label. *)
+          effect s vs (Label (LENGTH ts) [] ([], (MAP Plain es')))
+
+        (* 4.4.5.4 *)
+        | vs, Loop ts es' =>
+          (* Same stack and result length, loop is swapped for label. *)
+          effect s vs (Label 0 [pe] ([], (MAP Plain es')))
+
+        (* 4.4.5.5 *)
+        | V_i32 0w :: vs', If t i1s i2s =>
+          effect s vs' (Plain (Block t i2s))
+        | V_i32 i :: vs', If t i1s i2s =>
+          effect s vs' (Plain (Block t i1s))
+
+        (* 4.4.5.6 *)
+        | vs, Br k =>
+          effect s [] (Breaking (w2n k) vs)
+
+        (* 4.4.5.7 *)
+        | V_i32 0w :: vs', Br_if l =>
+          resulting s vs'
+        | V_i32 i :: vs', Br_if l =>
+          effect s vs' (Plain (Br l))
+
+        (* 4.4.5.8 *)
+        | V_i32 i :: vs', Br_table ls ln =>
+          let nls = to_list ls in
+          effect s vs' (Plain (Br (if w2n i < LENGTH nls then EL (w2n i) nls else ln)))
+
+        (* 4.4.5.9 *)
+        | vs, Return =>
+          effect s [] (Returning vs)
+
+        (* 4.4.5.10 *)
+        | vs, Call x =>
+          typ_assert "4.4.5.10.2" ((w2n x) < LENGTH s.frame.module.funcaddrs)
+            (effect s vs (Invoke (EL (w2n x) s.frame.module.funcaddrs)))
+
+        (* 4.4.5.11 *)
+        | V_i32 i :: vs', Call_indirect x =>
+          let tab = get_table s.store s.frame in
+            typ_assert "4.4.4.5.11.10" ((w2n x) < LENGTH tab)
+              (case EL (w2n i) tab of
+                | NONE => (SOME (TypeError "4.4.5.11.11"), s)
+                | SOME a =>
+                  typ_assert "4.4.5.11.13" (a < LENGTH s.store.funcs)
+                    if funcinst_type (EL a s.store.funcs) <> (EL (w2n x) s.frame.module.types)
+                    then (SOME (Trap "4.4.5.11.16"), s)
+                    else effect s vs' (Invoke a)
+              )
+
+        | vs, pe =>
+          evaluate_nomatch s
+      )
+
+      (* 4.4.5.6 *)
+      | vs, Label n is (vs', Breaking 0 r :: es') =>
+        expand s ((TAKE n r) ++ vs) (MAP Plain is)
+      | vs, Label n is (vs', Breaking k r :: es') =>
+        effect s vs (Breaking (k - 1) r)
+
+      (* 4.4.5.9 *)
+      | vs, Label n is (vs', Returning r :: es') =>
+        effect s vs (Returning r)
+      | vs, Frame n f (vs', Returning r :: es') =>
+        (NONE, s with code := ((TAKE n r) ++ vs, []))
+
+      (* 4.4.6.2 *)
+      (* Fall through from a label that has been fully reduced. *)
+      | vs, Label n is (vs', []) =>
+        resulting s (vs' ++ vs)
+
+      (* Recursion to evaluate what's inside a frame. *)
+      | vs, Frame n f c =>
+        (case evaluate_small (s with <| code := c; frame := f |>) of
+          | SOME r, s' => (SOME r, s')
+          | NONE  , s' => effect s vs (Frame n s'.frame s'.code)
+        )
+
+      (* Recursion to evaluate what's inside a label. *)
+      | vs, Label n is c =>
+        (case evaluate_small (s with code := c) of
+          | SOME r, s' => (SOME r, s')
+          | NONE  , s' => effect s vs (Label n is s'.code)
+        )
+
+      | vs, Breaking k r =>
+        (SOME (TypeError "Undefined label"), s)
+
+      (* 4.4.7.{1,3} *)
+      | vs, Invoke a =>
+        typ_assert "4.4.7.1.2" (a <= LENGTH s.store.funcs)
+          (case (EL a s.store.funcs) of
+            (* 4.4.7.1 *)
+            | Native (Tf t1 t2) mi f => (
+              let (n, m) = (LENGTH t1, LENGTH t2) in
+              typ_assert "4.4.7.1.{4,7} (at least one of the two)" (m <= 1 /\ n <= LENGTH vs)
+                (effect s (DROP n vs) (Frame
+                  m
+                  <| module := mi; locals := (TAKE n vs) ++ (MAP zero f.locals) |>
+                  ([], [Plain (Block t2 (expr_to_instrs f.body))])
+                ))
+            )
+
+            | _ => (SOME (TypeError "TODO TODO TODO"), s)
+            (* 4.4.7.3 *)
+            (* NOTE: We assume that any host function is of type [i32] ^ 4 -> []. *)
+            (* TODO: This case explodes. Assert i32^4 separately. *)
+            (* | Host (ForeignFunction name) => (case vs of *)
+            (*   | V_i32 (n2w len2) :: V_i32 (n2w ptr2) :: V_i32 (n2w len1) :: V_i32 (n2w ptr1) :: vs' => *)
+            (*     let rbs = read_mem s.store s.frame in *)
+            (*    case (rbs ptr1 len1, rbs ptr2 len2) of *)
+            (*       | SOME b1s, SOME b2s => (case call_FFI s.ffi name b1s b2s of *)
+            (*         | FFI_final outcome => (SOME (FinalFFI outcome), s) *)
+            (*         | FFI_return new_ffi new_bytes => (case write_mem s.store s.frame ptr1 new_bytes of *)
+            (*           | SOME s' => resulting (s with <| ffi := new_ffi; store := s' |>) vs' *)
+            (*           | NONE    => (SOME (Trap "Host function wants to write out of bounds"), s) *)
+            (*         ) *)
+            (*       ) *)
+            (*       | _ => (SOME (Trap "Host function arguments out of bounds"), s) *)
+            (*   | _ => (SOME (TypeError "Host function expects four i32 arguments"), s) *)
+            (* ) *)
+          )
+
+      (* 4.4.7.2 *)
+      | vs, Frame n f (vs', []) =>
+        resulting s (vs' ++ vs)
+
+      | vs, es =>
+        evaluate_nomatch s
+`
+(
+  WF_REL_TAC `inv_image ($< LEX $<) (\s. (s.clock, ainstr2_size (SND s.code)))` >>
+  simp [wasmSemanticPrimitivesTheory.ainstr_size_def]
+)
+
+val evaluate_small_progress = Q.store_thm("evaluate_small_progress",
+  `!s s'. evaluate_small s = (NONE, s') ==> inv_image ($< LEX $<) (\s. (s.clock, ainstr2_size (SND s.code))) s' s`,
+  ho_match_mp_tac (theorem "evaluate_small_ind") >> rpt gen_tac >> strip_tac >>
+  Cases_on `s.code` >> rename [`s.code = (vs, es)`] >>
+  Cases_on `es` >> ONCE_REWRITE_TAC [evaluate_small_def] >> simp [] >> rename [`s.code = (vs, e :: es)`] >>
+  Cases_on `e` >> simp []
+  >- (simp_tac (srw_ss () ++ boolSimps.COND_elim_ss) [AllCaseEqs (), PULL_EXISTS] >> rw[resulting_def,effect_def] >> TRY (drule expand_dec) >> simp [])
+  >- (simp [AllCaseEqs ()] >> rw[effect_def] >> (drule expand_dec) >> simp [])
+  >- (simp [AllCaseEqs ()] >> rw[effect_def,resulting_def] >> TRY (drule expand_dec) >> simp [])
+  >- (simp [AllCaseEqs ()] >> rw[effect_def,resulting_def] >> TRY (drule expand_dec) >> simp[wasmSemanticPrimitivesTheory.ainstr_size_def,pairTheory.LEX_DEF])
+)
 
 val evaluate_wasm_def = tDefine "evaluate_wasm" `
   evaluate_wasm s = case s.code of
@@ -340,10 +402,18 @@ val evaluate_wasm_def = tDefine "evaluate_wasm" `
       | NONE   , s' => evaluate_wasm s'
 `
 (
-  WF_REL_TAC `inv_image ($< LEX $< LEX $<) (\s. (s.clock, LENGTH (FST s.code), LENGTH (SND s.code)))` >>
-  REWRITE_TAC[evaluate_small_def] >> rpt strip_tac >> rfs [] >>
-  cheat
+  WF_REL_TAC `inv_image ($< LEX $<) (\s. (s.clock, ainstr2_size (SND s.code)))` >> rw [] >> drule evaluate_small_progress >> simp[wasmSemanticPrimitivesTheory.ainstr_size_def,pairTheory.LEX_DEF]
 )
+
+(* val evaluate_fill_b = Q.store_thm("evaluate_fill_b", *)
+(*   `(s.code = ([], Label (LENGTH vs) is (fill_b l holed (vs, [Plain (Br (n2w l))])))) ==> ((SOME vs, s') = evaluate_wasm s)`, *)
+(*   cheat *)
+(* ) *)
+
+(* val evaluate_fill_e = Q.store_thm("evaluate_fill_e", *)
+(*   `(s.code = ([], Frame (LENGTH vs) f (fill_e holed (vs, [Plain Return])))) ==> ((SOME vs, s') = evaluate_wasm s)`, *)
+(*   cheat *)
+(* ) *)
 
 (* TODO: Do we need something like evaluate_expression? *)
 
